



DEPARTMENT OF MATHEMATICS

CIE-II Scheme and Solution

Academic year 2025-2026 (Third Semester BE)

LINEAR ALGEBRA AND PROBABILITY THEORY (MA231TC)

(Common to CS, CD, CY, IS)

Q. No's	Question	M
PART A		
1	$k = -2$	1
2	6, 2	2
3	$\begin{bmatrix} 3 & 1 \\ 1 & 3 \end{bmatrix}$	2
4	$\ f\ = \sqrt{\int_0^2 f(x)f(x)dx} = \sqrt{\frac{32}{5}}$	2
5	$\frac{3+3k}{10} = 1 \Rightarrow k = \frac{7}{3}$	1
6	$\int_0^{\frac{1}{2}} kx dx = \frac{1}{4} \Rightarrow k = 2$	2
PART B		
1a	<p>Given vectors are $x_1 = (1,1,1,1)$, $x_2 = (1,-1,2,2)$, $x_3 = (1,2,-3,-4)$</p> <p>Steps of Gram-Schmidt method:</p> <p>$v_1 = x_1 = (1,1,1,1)$</p> <p>$v_2 = x_2 - \left(\frac{x_2 \cdot v_1}{v_1 \cdot v_1}\right) v_1$</p> <p>$v_2 = (1,-1,2,2) - \frac{(1,-1,2,2) \cdot (1,1,1,1)}{(1,1,1,1) \cdot (1,1,1,1)} (1,1,1,1) = (0,-2,1,1)$</p> <p>$v_3 = x_3 - \left(\frac{x_3 \cdot v_1}{v_1 \cdot v_1}\right) v_1 - \left(\frac{x_3 \cdot v_2}{v_2 \cdot v_2}\right) v_2$</p> <p>$v_3 = (1,2,-3,-4) - \frac{(1,2,-3,-4) \cdot (1,1,1,1)}{(1,1,1,1) \cdot (1,1,1,1)} (1,1,1,1) - \frac{(1,2,-3,-4) \cdot (0,-2,1,1)}{(0,-2,1,1) \cdot (0,-2,1,1)} (0,-2,1,1)$</p> <p>$= (2, -\frac{2}{3}, -\frac{1}{6}, -\frac{7}{6})$</p> <p>$Proj(v, S) = \left(\frac{v \cdot v_1}{v_1 \cdot v_1}\right) v_1 + \left(\frac{v \cdot v_2}{v_2 \cdot v_2}\right) v_2 + \left(\frac{v \cdot v_3}{v_3 \cdot v_3}\right) v_3 \Rightarrow \left(-\frac{1}{5}, \frac{12}{5}, \frac{3}{5}, \frac{6}{5}\right)$</p>	1 <

	$Q = \begin{bmatrix} \frac{1}{2} & \frac{3\sqrt{5}}{10} & -\frac{\sqrt{6}}{6} \\ -\frac{1}{2} & \frac{3\sqrt{5}}{10} & 0 \\ -\frac{1}{2} & \frac{\sqrt{5}}{10} & \frac{\sqrt{6}}{6} \\ \frac{1}{2} & \frac{\sqrt{5}}{10} & \frac{\sqrt{6}}{3} \end{bmatrix} \quad R = Q^T A = \begin{bmatrix} 2 & 1 & \frac{1}{2} \\ 0 & \sqrt{5} & \frac{3\sqrt{5}}{2} \\ 0 & 0 & \frac{\sqrt{6}}{2} \end{bmatrix}$	1 2
3	$\begin{vmatrix} 2-\lambda & 2 & 0 \\ 2 & 5-\lambda & 0 \\ 0 & 0 & 3-\lambda \end{vmatrix} = 0 \Rightarrow \lambda^3 - 10\lambda^2 + 27\lambda - 18 = 0.$ <p>Eigen values are 6, 3, 1</p> <p>Eigen vector corresponding to $\lambda = 6 \Rightarrow X_1 = \begin{bmatrix} 1 \\ 2 \\ 0 \end{bmatrix}$</p> <p>Eigen vector corresponding to $\lambda = 3 \Rightarrow X_2 = \begin{bmatrix} 0 \\ 0 \\ 1 \end{bmatrix}$</p> <p>Eigen vector corresponding to $\lambda = 1 \Rightarrow X_3 = \begin{bmatrix} -2 \\ 1 \\ 0 \end{bmatrix}$</p> <p>$\therefore$ Orthogonal matrix $P = \begin{bmatrix} \frac{1}{\sqrt{5}} & 0 & \frac{-2}{\sqrt{5}} \\ \frac{2}{\sqrt{5}} & 0 & \frac{1}{\sqrt{5}} \\ 0 & 1 & 0 \end{bmatrix}$ and $D = \begin{bmatrix} 6 & 0 & 0 \\ 0 & 3 & 0 \\ 0 & 0 & 1 \end{bmatrix}$.</p>	2 2 2 2 1 1
4	$AA^T = \begin{bmatrix} 3 & 2 & 2 \\ 2 & 3 & -2 \end{bmatrix} \begin{bmatrix} 3 & 2 \\ 2 & 3 \\ 2 & -2 \end{bmatrix} = \begin{bmatrix} 17 & 8 \\ 8 & 17 \end{bmatrix}$ <p>Eigen values of $AA^T = \begin{bmatrix} 17 & 8 \\ 8 & 17 \end{bmatrix}$ are 25 and 9.</p> $A^T A = \begin{bmatrix} 3 & 2 \\ 2 & 3 \\ 2 & -2 \end{bmatrix} \begin{bmatrix} 3 & 2 & 2 \\ 2 & 3 & -2 \end{bmatrix} = \begin{bmatrix} 13 & 12 & 2 \\ 12 & 13 & -2 \\ 2 & -2 & 8 \end{bmatrix}$ <p>Eigen values of $A^T A = \begin{bmatrix} 13 & 12 & 2 \\ 12 & 13 & -2 \\ 2 & -2 & 8 \end{bmatrix}$ are 25, 9 and 0.</p> <p>Eigen vectors of AA^T are $\begin{bmatrix} 1 \\ 1 \end{bmatrix}$ and $\begin{bmatrix} -1 \\ 1 \end{bmatrix}$</p> <p>Eigen vectors of $A^T A$ are $\begin{bmatrix} 1 \\ 1 \\ 0 \end{bmatrix}$, $\begin{bmatrix} -1 \\ 1 \\ -4 \end{bmatrix}$ and $\begin{bmatrix} -2 \\ 2 \\ 1 \end{bmatrix}$</p> <p>Hence singular value decomposition is.</p> $\begin{bmatrix} \frac{1}{\sqrt{2}} & -\frac{1}{\sqrt{2}} \\ \frac{1}{\sqrt{2}} & \frac{1}{\sqrt{2}} \end{bmatrix} \begin{bmatrix} 5 & 0 & 0 \\ 0 & 3 & 0 \end{bmatrix} \begin{bmatrix} \frac{1}{\sqrt{2}} & \frac{1}{\sqrt{2}} & 0 \\ -\frac{1}{\sqrt{18}} & \frac{1}{\sqrt{18}} & \frac{-4}{\sqrt{18}} \\ -\frac{2}{3} & \frac{2}{3} & \frac{1}{3} \end{bmatrix}$	2 1 2 2 3 2 1
5a	<p>$P(x) \geq 0$, for all x and $\sum p(x) = \frac{1}{2} \left\{ \left(\frac{2}{3}\right) + \left(\frac{2}{3}\right)^2 + \left(\frac{2}{3}\right)^3 + \dots \right\} = \frac{1}{2} \left\{ \frac{\frac{2}{3}}{1-\frac{2}{3}} \right\} = 1.$</p> <p>$P(X=x)$ is a probability distribution function.</p> <p>$P(X = \text{even}) = \frac{1}{2} \left\{ \left(\frac{2}{3}\right)^2 + \left(\frac{2}{3}\right)^4 + \dots \right\} = \frac{2}{5}.$</p>	2 2
5b	<p>The cumulative density function is given by</p> $F(x) = \begin{cases} 0, & x \leq 0 \\ \int_0^x (1-x) dx, & 0 < x < 1 \\ \int_0^1 (1-x) dx + \int_1^x x - 1 dx, & 1 < x < 2 \\ 1, & x > 2. \end{cases} \Rightarrow F(x) = \begin{cases} 0, & x \leq 0 \\ x - \frac{x^2}{2}, & 0 < x < 1 \\ \frac{x^2}{2} - x + 1, & 1 < x < 2 \\ 1, & x > 2. \end{cases}$ <p>$P(X > 1.4) = 1 - F(X \leq 1.4) = 1 - 0.58 = 0.42.$</p>	1 2 2 2